

Regression [in the population]

$$\left[\begin{array}{l} \text{given linear model } Y_i = \alpha + \beta X_i + \epsilon_i \\ \alpha, \beta \text{ s.t. } E(\epsilon_i) = 0 \quad E(\epsilon_i X_i) = 0 \end{array} \right]$$

① $\alpha, \beta = \underset{a, b}{\operatorname{argmin}} E \{ \underbrace{Y_i - [a + bX_i]} \}^2$ ① $\alpha + \beta X_i$ is the best linear predictor of Y_i

$$\frac{\partial \text{MSE}}{\partial a} = -2 E \{ Y_i - a - bX_i \} = 0$$
$$\Leftrightarrow E(\epsilon_i) = 0$$

$$\frac{\partial \text{MSE}}{\partial b} = -2 E \{ Y_i - a - bX_i \} X_i = 0$$
$$\Leftrightarrow E(X_i \epsilon_i) = 0$$

② if CEF is linear, then regression is the CEF

$$E[Y_i | X_i] = \alpha + \beta X_i$$
$$\epsilon_i = Y_i - E[Y_i | X_i]$$

$$E[\epsilon_i | X_i] = 0$$

$$E[\epsilon_i] = E[E[\epsilon_i | X_i]] = 0$$
$$E[X_i \epsilon_i] = E[X_i E[\epsilon_i | X_i]] = 0$$

② if the CEF is linear, then $\alpha + \beta X_i$ is the CEF

③ it's the best linear approx to CEF ③ even if the CEF is not linear, $\alpha + \beta X_i$ is the best linear approx. to it

$$\rightarrow (\alpha, \beta) = \underset{a, b}{\operatorname{argmin}} E \{ [E[Y_i | X_i] - (\alpha + bX_i)]^2 \}$$

OLS [In the data]

$$(\hat{\alpha}_{OLS}, \hat{\beta}_{OLS}) = \underset{a, b}{\operatorname{argmin}} \sum_i (y_i - a - bx_i)^2$$

$$\hat{\beta}_{OLS} = \frac{s_{xy}}{s_x^2}$$

$$E[\hat{\beta}_{OLS}] = \beta? \quad \text{is } \hat{\beta}_{OLS} \text{ an unbiased estimator of } \beta?$$

$$\begin{aligned} \hat{\beta}_{OLS} &= \frac{s_{xy}}{s_x^2} = \frac{\sum (x_i - \bar{x})(y_i - \bar{y})}{\sum (x_i - \bar{x})^2} \cdot \frac{1}{\cancel{n-1}} \quad \begin{array}{l} \xrightarrow{\sum (x_i - \bar{x}) y_i - \bar{y} \sum (x_i - \bar{x})} \\ \xrightarrow{\sum [(x_i - \bar{x}) y_i - (x_i - \bar{x}) \bar{y}]} \end{array} \\ &= \frac{\sum (x_i - \bar{x}) y_i}{\sum (x_i - \bar{x}) x_i} \quad \begin{array}{l} \xrightarrow{\sum (x_i - \bar{x}) y_i - \bar{y} \sum (x_i - \bar{x})} \\ \xrightarrow{\sum x_i - n\bar{x}} \end{array} \end{aligned}$$

$$= \frac{\sum (x_i - \bar{x}) [\alpha + \beta x_i + \varepsilon_i]}{\sum (x_i - \bar{x}) x_i}$$

$$= \alpha \underbrace{\frac{\sum (x_i - \bar{x})}{\sum (x_i - \bar{x}) x_i}}_0 + \beta \underbrace{\frac{\sum (x_i - \bar{x}) x_i}{\sum (x_i - \bar{x}) x_i}}_1 + \frac{\sum (x_i - \bar{x}) \varepsilon_i}{\sum (x_i - \bar{x}) x_i}$$

$$\hat{\beta}_{OLS} = \beta + \frac{\sum (x_i - \bar{x}) \varepsilon_i}{\sum (x_i - \bar{x}) x_i}$$

$$E[\beta_{OLS}] = \beta$$

$$E[\hat{\beta}_{OLS}] = E\left[\beta + \frac{\sum (x_i - \bar{x}) \varepsilon_i}{\sum (x_i - \bar{x}) x_i}\right]$$

ass: x_i is fixed

$$\sum x_i \varepsilon_i - \bar{x} \sum \varepsilon_i \neq 0$$

in a given sample, this does not need to be true!

$$= \beta + E\left[\frac{\sum (x_i - \bar{x}) \varepsilon_i}{\sum (x_i - \bar{x}) x_i}\right]$$

$$= \beta + \frac{\sum (x_i - \bar{x}) E[\varepsilon_i]}{\sum (x_i - \bar{x}) x_i} = 0$$

$$E[\hat{\beta}_{OLS}] = \beta + E\left[\frac{\sum (x_i - \bar{x}) \varepsilon_i}{\sum (x_i - \bar{x}) x_i}\right]$$

$$E\left[E\left[\frac{\sum (x_i - \bar{x}) \varepsilon_i}{\sum (x_i - \bar{x}) x_i} \mid x_i\right]\right]$$

$$E\left[\frac{\sum (x_i - \bar{x}) E[\varepsilon_i | x_i]}{\sum (x_i - \bar{x}) x_i}\right]$$

$$\begin{aligned} E(\varepsilon_i) &\neq E(\varepsilon_i | x_i) = 0 \\ E(\varepsilon_i | x_i) = 0 &\Rightarrow E(\varepsilon_i' x_i) = 0 \end{aligned}$$

$$\begin{aligned} E(Y_i - \alpha - \beta x_i | x_i) &= 0 \\ &= E[Y_i | x_i] \end{aligned}$$

ass: CEF is linear

Regression anatomy

$$Y_i = \beta_0 + \beta_1 X_{1i} + \beta_2 X_{2i} + \varepsilon_i$$

$$X_{1i} = \underbrace{\delta_0 + \delta_{12} X_{2i}}_{=\hat{X}_{1i} \text{ (fitted values)}} + \underbrace{\tilde{x}_{1i}}_{\text{residuals}}$$

$$E[\hat{X}_{1i} \tilde{x}_{1i}] = 0$$

$$\text{since } E[\tilde{x}_{1i}] = 0$$

$$\text{and } E[X_{2i} \tilde{x}_{1i}] = 0$$

{ regression residual
uncorrelated with the
regressors that made them }

$$\beta_1 = \frac{\text{cov}(Y_i, \tilde{x}_{1i})}{V(\tilde{x}_{1i})}$$

$$\text{cov}(Y_i, \tilde{x}_{1i}) = E[(\beta_0 + \beta_1 X_{1i} + \beta_2 X_{2i} + \varepsilon_i) \tilde{x}_{1i}]$$

$$= E[\beta_0 \tilde{x}_{1i}] = \beta_0 E[\tilde{x}_{1i}] = 0$$

$$+ \beta_1 E[X_{1i} \tilde{x}_{1i}] \rightarrow \beta_1 [E[(\hat{X}_{1i} + \tilde{x}_{1i})(\tilde{x}_{1i})]] = \beta_1 V(\tilde{x}_{1i})$$

$$+ \beta_2 E[X_{2i} \tilde{x}_{1i}]$$

$$+ E[\varepsilon_i \tilde{x}_{1i}] = 0$$

$$E(\hat{X}_{1i} \tilde{x}_{1i}) + E[\tilde{x}_{1i}^2]$$

$$= \delta_0 + \delta_{12} X_{2i} = 0$$

$$V(\tilde{x}_{1i})$$

$$E[\varepsilon_i (X_{1i} - \delta_0 - \delta_{12} X_{2i})]$$

$$V(x) = E[x^2] - [E(x)]^2$$

$$\text{cov}(Y_i, \tilde{x}_{1i}) = \beta_1 \text{var}(\tilde{x}_{1i})$$

$$\text{In the pret: } \frac{\text{cov}(\tilde{Y}_i, \tilde{x}_{1i})}{V(\tilde{x}_{1i})} = \beta_1$$

$$Y_i = \alpha_1 + \alpha_{12} X_{2i} + \tilde{Y}_i$$